proof/infoflow/RISCV64/ArchIpc_IF.thy
@@ -36,24 +36,25 @@ lemma storeWord_equiv_but_for_labels[Ipc_IF_assms]:
   apply (wp modify_wp)
   apply (clarsimp simp: equiv_but_for_labels_def)
   apply (rule states_equiv_forI)
-          apply (fastforce intro!: equiv_forI elim!: states_equiv_forE dest: equiv_forD)
-         apply (simp add: states_equiv_for_def)
-         apply (rule conjI)
-          apply (rule equiv_forI)
-          apply clarsimp
-          apply (drule_tac f=underlying_memory in equiv_forD,fastforce)
-          apply (fastforce intro: is_aligned_no_wrap' word_plus_mono_right
-                            simp: is_aligned_mask for_each_byte_of_word_def word_size_def upto.simps)
-         apply (rule equiv_forI)
-         apply clarsimp
-         apply (drule_tac f=device_state in equiv_forD,fastforce)
-         apply clarsimp
-        apply (fastforce elim: states_equiv_forE intro: equiv_forI dest: equiv_forD[where f=cdt])
-       apply (fastforce elim: states_equiv_forE intro: equiv_forI dest: equiv_forD[where f=cdt_list])
-      apply (fastforce elim: states_equiv_forE intro: equiv_forI dest: equiv_forD[where f=is_original_cap])
-     apply (fastforce elim: states_equiv_forE intro: equiv_forI dest: equiv_forD[where f=interrupt_states])
-    apply (fastforce elim: states_equiv_forE intro: equiv_forI dest: equiv_forD[where f=interrupt_irq_node])
-   apply (fastforce simp: equiv_asids_def equiv_asid_def elim: states_equiv_forE)
+            apply (fastforce intro!: equiv_forI elim!: states_equiv_forE dest: equiv_forD)
+           apply (simp add: states_equiv_for_def)
+           apply (rule conjI)
+            apply (rule equiv_forI)
+            apply clarsimp
+            apply (drule_tac f=underlying_memory in equiv_forD,fastforce)
+            apply (fastforce intro: is_aligned_no_wrap' word_plus_mono_right
+                              simp: is_aligned_mask for_each_byte_of_word_def word_size_def upto.simps)
+           apply (rule equiv_forI)
+           apply clarsimp
+           apply (drule_tac f=device_state in equiv_forD,fastforce)
+           apply clarsimp
+          apply (fastforce elim: states_equiv_forE intro: equiv_forI dest: equiv_forD[where f=cdt])
+         apply (fastforce elim: states_equiv_forE intro: equiv_forI dest: equiv_forD[where f=cdt_list])
+        apply (fastforce elim: states_equiv_forE intro: equiv_forI dest: equiv_forD[where f=is_original_cap])
+       apply (fastforce elim: states_equiv_forE intro: equiv_forI dest: equiv_forD[where f=interrupt_states])
+      apply (fastforce elim: states_equiv_forE intro: equiv_forI dest: equiv_forD[where f=interrupt_irq_node])
+     apply (fastforce simp: equiv_asids_def equiv_asid_def elim: states_equiv_forE)
+    apply auto[2]
   apply (fastforce elim: states_equiv_forE intro: equiv_forI dest: equiv_forD[where f=ready_queues])
   done
 
@@ -202,24 +203,22 @@ lemma dmo_loadWord_reads_respects[Ipc_IF_assms]:
   "reads_respects aag l (K (for_each_byte_of_word (\<lambda> x. aag_can_read_or_affect aag l x) p))
                   (do_machine_op (loadWord p))"
   apply (rule gen_asm_ev)
-  apply (rule use_spec_ev)
-  apply (rule spec_equiv_valid_hoist_guard)
-  apply (rule do_machine_op_spec_reads_respects)
-   apply (simp add: loadWord_def equiv_valid_def2 spec_equiv_valid_def)
-   apply (rule_tac R'="\<lambda>rv rv'. for_each_byte_of_word (\<lambda>y. rv y = rv' y) p"
-               and Q="\<top>\<top>" and Q'="\<top>\<top>" and P="\<top>" and P'="\<top>" in equiv_valid_2_bind_pre)
-        apply (rule_tac R'="(=)" and Q="\<lambda> r s. p && mask 3 = 0" and Q'="\<lambda> r s. p && mask 3 = 0"
-                    and P="\<top>" and P'="\<top>" in equiv_valid_2_bind_pre)
-             apply (rule return_ev2)
-             apply (rule_tac f="word_rcat" in arg_cong)
-             apply (fastforce simp: upto.simps is_aligned_mask for_each_byte_of_word_def word_size_def
-                             intro: is_aligned_no_wrap' word_plus_mono_right)
-            apply (rule assert_ev2[OF refl])
-           apply (rule assert_wp)+
-         apply simp+
-       apply (clarsimp simp: equiv_valid_2_def in_monad for_each_byte_of_word_def)
-       apply (fastforce elim: equiv_forD orthD1 simp: ptr_range_def add.commute)
-      apply (wp wp_post_taut loadWord_inv | simp)+
+  apply (rule do_machine_op_reads_respects)
+     apply (simp add: loadWord_def equiv_valid_def2 spec_equiv_valid_def)
+     apply (rule_tac R'="\<lambda>rv rv'. for_each_byte_of_word (\<lambda>y. rv y = rv' y) p"
+                 and Q="\<top>\<top>" and Q'="\<top>\<top>" and P="\<top>" and P'="\<top>" in equiv_valid_2_bind_pre)
+          apply (rule_tac R'="(=)" and Q="\<lambda> r s. p && mask 3 = 0" and Q'="\<lambda> r s. p && mask 3 = 0"
+                      and P="\<top>" and P'="\<top>" in equiv_valid_2_bind_pre)
+               apply (rule return_ev2)
+               apply (rule_tac f="word_rcat" in arg_cong)
+               apply (fastforce simp: upto.simps is_aligned_mask for_each_byte_of_word_def word_size_def
+                               intro: is_aligned_no_wrap' word_plus_mono_right)
+              apply (rule assert_ev2[OF refl])
+             apply (rule assert_wp)+
+           apply simp+
+         apply (clarsimp simp: equiv_valid_2_def in_monad for_each_byte_of_word_def)
+         apply (fastforce elim: equiv_forD orthD1 simp: ptr_range_def add.commute)
+        apply (wp wp_post_taut loadWord_inv | simp)+
   done
 
 lemma complete_signal_reads_respects[Ipc_IF_assms]:
@@ -287,7 +286,7 @@ global_interpretation Ipc_IF_1?: Ipc_IF_1
 proof goal_cases
   interpret Arch .
   case 1 show ?case
-    by (unfold_locales; (fact Ipc_IF_assms)?)
+    by (unfold_locales; (fact Ipc_IF_assms | wpsimp wp: Ipc_IF_assms)?)
 qed
 
 
@@ -441,7 +440,7 @@ lemma set_mrs_reads_respects'[Ipc_IF_assms]:
   apply (simp add: equiv_valid_def2)
   apply (rule equiv_valid_rv_guard_imp)
    apply (case_tac buf)
-    apply (rule_tac Q="\<top>" and P="\<top>" and L="{pasObjectAbs aag thread}" in ev_invisible[OF domains_distinct])
+    apply (rule_tac Q="\<top>" and P="\<top>" and L="{pasObjectAbs aag thread}" in revrv_invisible[OF domains_distinct])
       apply (clarsimp simp: labels_are_invisible_def)
      apply (rule modifies_at_mostI)
      apply (simp add: set_mrs_def)
@@ -451,7 +450,7 @@ lemma set_mrs_reads_respects'[Ipc_IF_assms]:
    apply (rename_tac buf')
    apply (rule_tac Q="\<top>" and L="{pasObjectAbs aag thread} \<union> (pasObjectAbs aag)
                                  ` (ptr_range buf' msg_align_bits)"
-                in ev_invisible[OF domains_distinct])
+                in revrv_invisible[OF domains_distinct])
      apply (auto simp: labels_are_invisible_def ipc_buffer_has_auth_def
                  dest: reads_read_page_read_thread simp: aag_can_affect_label_def)[1]
     apply (rule modifies_at_mostI)
